Add Simple stepsl_to_eval

proof/Simple/EsJudge.v
@@ -4,6 +4,8 @@ Require Export SubstValueValue.
 
 
 (* Single Small Step Evaluation *************************************
+   The single step rules model the individual transitions that the 
+   machine can make at runtime.
  *)
 Inductive STEP : exp -> exp -> Prop :=
  | ESLamApp
@@ -27,45 +29,31 @@ Hint Constructors STEP.
 
 
 (* Multi-step evaluation *******************************************
-   This is a sequence of small step evaluations.
+   A sequence of small step transitions.
  *)
-Inductive STEPS : nat -> exp -> exp -> Prop :=
+Inductive STEPS : exp -> exp -> Prop :=
 
  (* After no steps, we get the same exp.
-    We need this constructor to match the EVValue constructor
+    We need this constructor to match the EVDone constructor
     in the big-step evaluation, so we can convert between big-step
-    and mult-step evaluations. *)
- | ESDone
+    and multi-step evaluations. *)
+ | ESNone
    :  forall x1
-   ,  STEPS 0 x1 x1
+   ,  STEPS x1 x1
 
  (* Take a single step. *)
  | ESStep
    :  forall x1 x2
    ,  STEP  x1 x2
-   -> STEPS 1 x1 x2
+   -> STEPS x1 x2
 
- (* Combine two reductions into a third. *)
- | ESLink
-   :  forall n1 n2 x1 x2 x3
-   ,  STEPS n1 x1 x2 -> STEPS n2 x2 x3
-   -> STEPS (n1 + n2) x1 x3.
+ (* Combine two evaluations into a third. *)
+ | ESAppend
+   :  forall x1 x2 x3
+   ,  STEPS x1 x2 -> STEPS x2 x3
+   -> STEPS x1 x3.
 
 Hint Constructors STEPS.
-
-
-(* Left linearised multi-step evaluation ****************************)
-Inductive STEPSL : nat -> exp -> exp -> Prop :=
-
- | ESRefl 
-   : forall x1
-   , STEPSL 0 x1 x1
-
- | ESSnoc 
-   :  forall n x1 x2 x3
-   ,  STEPSL n x1 x2 
-   -> STEP   x2 x3
-   -> STEPSL (S n) x1 x3.
 
 
 (* Context lemmas ***************************************************
@@ -73,9 +61,9 @@ Inductive STEPSL : nat -> exp -> exp -> Prop :=
    context. They're all trivial.
  *)
 Lemma steps_app1
- :  forall n x1 x1' x2
- ,  STEPS n x1 x1'
- -> STEPS n (XApp x1 x2) (XApp x1' x2).
+ :  forall x1 x1' x2
+ ,  STEPS x1 x1'
+ -> STEPS (XApp x1 x2) (XApp x1' x2).
 Proof.
  intros. induction H; eauto.
 Qed.
@@ -83,12 +71,56 @@ Hint Resolve steps_app1.
 
 
 Lemma steps_app2
- :  forall n v1 x2 x2'
+ :  forall v1 x2 x2'
  ,  value v1 
- -> STEPS n x2 x2'
- -> STEPS n (XApp v1 x2) (XApp v1 x2').
+ -> STEPS x2 x2'
+ -> STEPS (XApp v1 x2) (XApp v1 x2').
 Proof.
  intros. induction H0; eauto.
 Qed.
 Hint Resolve steps_app2.
+
+
+(* Left linearised multi-step evaluation ****************************)
+Inductive STEPSL : exp -> exp -> Prop :=
+
+ | ESLNone 
+   : forall x1
+   , STEPSL x1 x1
+
+ | ESLSnoc 
+   :  forall x1 x2 x3
+   ,  STEP   x1 x2 -> STEPSL x2 x3 
+   -> STEPSL x1 x3.
+
+Hint Constructors STEPSL.
+
+
+(* Transitivity of left linearised multi-step evaluation. *)
+Lemma stepsl_trans
+ :  forall x1 x2 x3
+ ,  STEPSL x1 x2 -> STEPSL x2 x3
+ -> STEPSL x1 x3.
+Proof.
+ intros.
+ induction H.
+  eauto.
+  eapply ESLSnoc. eauto. eauto.
+Qed.
+
+
+(* Linearise a regular multi-step evaluation. *)
+Lemma steps_to_stepsl
+ :  forall x1 x2
+ ,  STEPS  x1 x2
+ -> STEPSL x1 x2.
+Proof. 
+ intros.
+ induction H.
+  auto.
+  eauto.
+  eapply stepsl_trans; eauto.
+Qed.
+  
+
 
